proof/SomeDKC.ec
@@ -20,30 +20,112 @@ require import GarbleTools.
 theory SomeDKC.
   clone import ExtWord as W.
   clone ExtWord as KW with op length = W.length - 1.
+
+  (*************************************)
+  (** AUXLIAR FUNCTIONS *)
+  (*************************************)
+  
+  op kw2w(kw,lsb) =
+  if kw = witness then witness else
+                   let lsbi = if lsb then 1 else 0
+                      in let kwi = (KW.to_int kw) * 2 + lsbi
+                      in W.setlsb (W.from_int kwi) lsb.
+
+  op kw2w'(kw,lsb) =
+                   let lsbi = if lsb then 1 else 0
+                      in let kwi = (KW.to_int kw) * 2 + lsbi
+                      in W.setlsb (W.from_int kwi) lsb.
+  
+  op w2kw(w) =
+  if w = witness then (witness,W.getlsb w) else
+  let kwi = (W.to_int w) %/ 2 (* / 2 *)
+                          in let lsbi = W.getlsb w
+                          in (KW.from_int kwi,lsbi).
+
+  op w2kw'(w) =
+  let kwi = (W.to_int w) %/ 2 (* / 2 *)
+                          in let lsbi = W.getlsb w
+                          in (KW.from_int kwi,lsbi).
+  
+  lemma w2kw_kw2w w b : fst (w2kw (kw2w w b)) = w. 
+  proof.
+    simplify w2kw kw2w fst.
+    case b => hc.
+    smt tmo=60.
+    simplify.
+    smt tmo=60.
+  qed.
+
+  lemma kw2w_w2kw w b :
+    getlsb w = b => kw2w (fst (w2kw w)) b = w.
+  proof.
+    move => hlsb.
+    simplify kw2w w2kw fst.
+    case b => hc.
+    smt tmo=60.
+    simplify.
+    smt tmo=60.
+  qed.
+
+  lemma kw2w_w2kw' w b :
+    getlsb w = b => kw2w (fst (w2kw' w)) b = w.
+  proof.
+    move => hlsb.
+    simplify kw2w w2kw' fst.
+    case b => hc.
+    smt tmo=60.
+    simplify.
+    smt tmo=60.
+  qed.
+  
+  lemma w2kw'_kw2w' w b : fst (w2kw' (kw2w' w b)) = w. 
+  proof.
+    simplify w2kw kw2w fst.
+    case b => hc.
+    smt tmo=60.
+    simplify.
+    smt tmo=60.
+  qed.
+
+  lemma kw2w'_w2kw' w b :
+    getlsb w = b => kw2w' (fst (w2kw' w)) b = w.
+  proof.
+    move => hlsb.
+    simplify kw2w w2kw fst.
+    case b => hc.
+    smt tmo=60.
+    simplify.
+    smt tmo=60.
+  qed.
+  
+  (*op w2kw'(w) =
+  (*if w = witness then witness else*)
+  let kwi = (W.to_int w) %/ 2 (* / 2 *)
+                          in let lsbi = W.getlsb w
+                          in KW.from_int kwi.*)
   
   clone import SomePRF.PRF with
 	type D = word,
 	type R = word,
-	type K = KW.word.
-
-  op E(t,k1,k2,m) = (F k1 t) ^ (F k2 t) ^ m.
-  op D(t,k1,k2,c) = (F k1 t) ^ (F k2 t) ^ c.
-
-  clone import DKC.DKC as PrfDKC with
+	type K = KW.word,
+        op dK = KW.Dword.dword.
+          
+  clone import DKC.DKCScheme as PrfDKC with
         type tweak_t = word,
         type msg_t = word,
-        type key1_t = KW.word,
-        type key2_t = KW.word,
+        type key1_t = word,
+        type key2_t = word,
         type cipher_t = word,
-        op E = E,
-        op D = D.
-
+        op E(t,k1,k2,m) = (F (fst (w2kw k1)) t) ^ (F (fst (w2kw k2)) t) ^ m,
+        op D(t,k1,k2,c) = (F (fst (w2kw k1)) t) ^ (F (fst (w2kw k2)) t) ^ c.
+        
   (*prover ["Z3"].*)
         
   (** DKC security definitions, instantiated with the words defined in W *)
   clone import DKCSec2.DKCSecurity with
-        theory WD <- W,
-        theory D <- PrfDKC.
+    (*theory WD <- W,*)
+        theory DKCScheme <- PrfDKC.
+  
 
   lemma PrfDKC_correct : PrfDKC.Correct().
   proof.
@@ -58,7 +140,100 @@ theory SomeDKC.
       repeat. *)
    
   (*op bound: int.*)
+  
+  (*************************************)
+  (** DKC PART *)
+  (*************************************)
+  
+  (** DKC parameters *)
+  module DKCp = {
+    var b : bool
+    var ksec : word
+    var kpub : ((int * bool), word) fmap
+    var used : word fset
+    var lsb : bool
+    var l : int
+  }.
+
+  op itb (x:int) = if x = 1 then true else false.
+  
+  module DKC_O : DKC_AdvOracles = {    
     
+    proc initialize(b : bool,l:int): bool = {
+      var i, tok1, tok2;
+      
+      DKCp.b = b;
+      DKCp.l = l;
+      DKCp.lsb = witness;
+      DKCp.used = FSet.fset0;
+      DKCp.kpub = map0;
+      
+      i = 0;
+      while (i < bound) {
+        DKCp.kpub.[(i, false)] = W.zeros;
+        DKCp.kpub.[(i, true)] = W.zeros;
+        i = i + 1;
+      }
+            
+      i = 0;
+      while (i < bound) {
+        if (i = DKCp.l) {
+          DKCp.lsb = ${0,1};
+          DKCp.kpub.[(i,DKCp.lsb)] = witness; (* can never return or encrypt this key *)
+          DKCp.kpub.[(i,!DKCp.lsb)] = $Dword.dwordLsb (!DKCp.lsb);  
+        }
+        else {
+          tok1 = $Dword.dwordLsb (false);
+          tok2 = $Dword.dwordLsb (true);
+            DKCp.kpub.[(i, false)] = tok1;
+            DKCp.kpub.[(i, true)] = tok2;
+        }
+        i = i + 1;
+      }
+
+      DKCp.ksec = $Dword.dwordLsb (DKCp.lsb);
+      
+      return DKCp.lsb;
+    }
+    
+    proc encrypt(q:query_DKC) : answer_DKC = {
+      var aa,bb,xx : word;
+      var ib,jb,lb : int * bool;
+      var bi,bj,bl', rn: bool;
+      var t, ki, kj : word;
+      var ans : answer_DKC;
+
+      ans = bad;
+      (rn,ib,jb,lb,t) = q;
+      
+      if (!(mem DKCp.used t) && 0 <= ib.`1 /\ ib.`1 < jb.`1 && jb.`1 < lb.`1 && lb.`1 < bound /\ lb <> (DKCp.l,DKCp.lsb)) {
+        DKCp.used = DKCp.used `|` fset1 t; (* to do: check unicity *)
+        
+        ki = oget DKCp.kpub.[ib];
+        kj = oget DKCp.kpub.[jb];
+        
+        (aa,bb) = if (ib = (DKCp.l,DKCp.lsb)) 
+                  then (DKCp.ksec, kj) 
+                  else (if (jb = (DKCp.l,DKCp.lsb)) 
+                        then (ki, DKCp.ksec) 
+                        else (ki,kj));
+
+        xx = oget DKCp.kpub.[lb];
+        
+        if (((((DKCp.l,DKCp.lsb) = ib) || ((DKCp.l,DKCp.lsb) = jb)) /\ !DKCp.b) || rn) {
+          xx = $Dword.dword;
+        }
+        ans = (ki, kj, E t aa bb xx);
+      }
+
+      return ans;
+    }
+  }.
+
+  (*************************************)
+  (** PRF PART *)
+  (*************************************)
+  
   module Param = {
     var kpub : ((int * bool), (KW.word * bool)) fmap
     var used : word fset
@@ -66,19 +241,6 @@ theory SomeDKC.
     var l : int
     var tbl : (word,word) fmap
   }.
-
-  op kw2w(kw,lsb) =
-  (*if kw = witness then witness else*)
-                   let lsbi = if lsb then 1 else 0
-                      in let kwi = (KW.to_int kw) * 2 + lsbi
-                      in W.setlsb (W.from_int kwi) lsb.
-
-  op w2kw(w) =
-  (*if w = witness then witness else*)
-  let kwi = (W.to_int w) %/ 2 (* / 2 *)
-                          in let lsbi = W.getlsb w
-                          in (KW.from_int kwi,lsbi).
-  
     
   module DKC_Oracle(O:PRF_Oracle) = {
     proc encrypt(q:query_DKC) : answer_DKC = {
@@ -95,7 +257,7 @@ theory SomeDKC.
       ans = bad;
       (rn,ib,jb,lb,t) = q;
   
-      if (!(mem Param.used t) && ib.`1 < jb.`1 && jb.`1 < lb.`1 && lb <> (Param.l,Param.lsb)) {
+      if (!(mem Param.used t) && 0 <= ib.`1 /\ ib.`1 < jb.`1 && jb.`1 < lb.`1 && lb.`1 < bound /\ lb <> (Param.l,Param.lsb)) {
         Param.used = Param.used `|` fset1 t; 
         
         (ki,lsbi) = oget Param.kpub.[ib];
@@ -113,12 +275,12 @@ theory SomeDKC.
           xx = $Dword.dword;
         }
         
-        if ((Param.l,Param.lsb)=ib) {
+        if (ib = (Param.l,Param.lsb)) {
           mask = O.f(t);
           ans = (kw2w ki lsbi, kw2w kj lsbj, mask ^ (F kj t) ^ xx);
         }
         else  {
-            if ((Param.l,Param.lsb)=jb) {
+            if (jb = (Param.l,Param.lsb)) {
               mask = O.f(t);
               ans = (kw2w ki lsbi, kw2w kj lsbj, (F ki t) ^ mask ^ xx);
            }
@@ -157,7 +319,7 @@ theory SomeDKC.
       while (i < bound) {
         if (i = Param.l) {
           Param.lsb = ${0,1};
-          Param.kpub.[(i,Param.lsb)] = witness; (* can never return or encrypt this key *)
+          Param.kpub.[(i,Param.lsb)] = (witness,Param.lsb); (* can never return or encrypt this key *)
           ki = $KW.Dword.dword;
           Param.kpub.[(i,!Param.lsb)] = (ki,(!Param.lsb));  
         }
@@ -183,83 +345,409 @@ theory SomeDKC.
   }.
       
   
-equiv true_key lp b (A <:  Adv_DKC_t):
-    DKCSecurity.Game(DKC,A).game ~
-    IND(PRFr_Wrapped,D(A)).main : 0 <= lp < boundl /\ b = true /\ l{1} = lp /\ l{2} = lp
+equiv true_key lp (A <:  Adv_DKC_t{Param,DKCp,PRFr_Wrapped}):
+    DKCSecurity.Game(DKC_O,A).game ~
+    IND(PRFr_Wrapped,D(A)).main : ={glob A} /\ 0 <= lp < bound /\ b{1} /\ l{1} = lp /\ l{2} = lp
                                ==> ={res}.
     proof.
       proc.
       inline PRFr_Wrapped.init D(A,PRFr_Wrapped).distinguish. 
-      seq 1 3 : (0 <= lp < boundl /\ b = true /\ (b{1}, l{1}).`2 = lp /\ l{2} = lp /\
-      DKCp.used{1} = Param.used{2} /\ DKCp.used{1} = fset0 /\
-      DKCp.l{1} = Param.l{2} /\ DKCp.l{1} = lp /\ 
-      DKCp.lsb{1} = Param.lsb{2} /\
+      seq 1 3 : (={glob A} /\ 0 <= lp < bound /\ b{1} /\ (b{1}, l{1}).`2 = lp /\ l{2} = lp /\
+      DKCp.used{1} = Param.used{2} /\ DKCp.used{1} = fset0 /\ DKCp.b{1} = b{1} /\ DKCp.b{1} /\
+      DKCp.l{1} = Param.l{2} /\ DKCp.l{1} = lp /\ Param.l{2} = l0{2} /\ DKCp.l{1} = l{1} /\
+      DKCp.lsb{1} = Param.lsb{2} /\ DKCp.ksec{1} = kw2w PRFr_Wrapped.k{2} Param.lsb{2} /\ getlsb DKCp.ksec{1} = DKCp.lsb{1} /\ lsb{1} = DKCp.lsb{1} /\ lsb{2} = Param.lsb{2} /\
       Param.tbl{2} = map0 /\
-      (forall k, 0 <= k < bound => k <> Param.l{2} => oget DKCp.kpub{1}.[(k,true)] = kw2w (fst (oget Param.kpub{2}.[(k,true)])) true) /\
-      (forall k, 0 <= k < bound => k <> Param.l{2} => oget DKCp.kpub{1}.[(k,false)] = kw2w (fst (oget Param.kpub{2}.[(k,false)])) false) /\
-      (forall k, 0 <= k < bound => k = Param.l{2} => oget DKCp.kpub{1}.[(k,!Param.lsb{2})] = kw2w (fst (oget Param.kpub{2}.[(k,!Param.lsb{2})])) (!Param.lsb{2})));   
-      inline DKC.initialize D(A, PRFr_Wrapped).initialize.
+
+      (*oget Param.kpub{2}.[(Param.l{2},Param.lsb{2})] = (witness,witness) /\
+      oget DKCp.kpub{1}.[(DKCp.l{1},DKCp.lsb{1})] = witness /\*)
+      oget DKCp.kpub{1}.[(DKCp.l{1},DKCp.lsb{1})] = kw2w (fst (oget Param.kpub{2}.[(Param.l{2},Param.lsb{2})])) Param.lsb{2} /\
+      (*snd (oget Param.kpub{2}.[(Param.l{2},Param.lsb{2})]) = Param.lsb{2} /\*)
+      (forall k b, 0 <= k < bound => k <> Param.l{2} => oget DKCp.kpub{1}.[(k,b)] = kw2w (fst (oget Param.kpub{2}.[(k,b)])) b) /\
+      (forall k b, 0 <= k < bound => snd (oget Param.kpub{2}.[(k,b)]) = b) /\
+      (forall k, 0 <= k < bound => k = Param.l{2} => oget DKCp.kpub{1}.[(k,!Param.lsb{2})] = kw2w (fst (oget Param.kpub{2}.[(k,!Param.lsb{2})])) (!Param.lsb{2}))
+
+
+
+    );   
+      inline DKC_O.initialize D(A, PRFr_Wrapped).initialize.
+
+        swap{2} 1 11.
+        wp. rnd (fun w, fst (w2kw' w)) (fun w, kw2w' w (Param.lsb{2})).
     
-        wp; while (0 <= lp < boundl /\ b = true /\ ={i} /\ 0 <= i{1} <= bound /\ (b{1}, l{1}).`2 = lp /\ l{2} = lp /\
-      DKCp.used{1} = Param.used{2} /\ DKCp.used{1} = fset0 /\
-      DKCp.l{1} = Param.l{2} /\ DKCp.l{1} = lp /\
-      DKCp.lsb{1} = Param.lsb{2} /\
-      Param.tbl{2} = map0 /\
-      (forall k, 0 <= k < i{1} => k <> Param.l{2} => oget DKCp.kpub{1}.[(k,true)] = kw2w (fst (oget Param.kpub{2}.[(k,true)])) true) /\
-      (forall k, 0 <= k < i{1} => k <> Param.l{2} => oget DKCp.kpub{1}.[(k,false)] = kw2w (fst (oget Param.kpub{2}.[(k,false)])) false) /\
+        wp; while (={glob A} /\ 0 <= lp < bound /\ b{1} /\ ={i} /\ 0 <= i{1} <= bound /\ (b{1}, l{1}).`2 = lp /\ l{2} = lp /\
+      DKCp.used{1} = Param.used{2} /\ DKCp.used{1} = fset0 /\ DKCp.b{1} = b{1} /\ DKCp.b{1} /\
+      DKCp.l{1} = Param.l{2} /\ DKCp.l{1} = lp /\ Param.l{2} = l0{2} /\ DKCp.l{1} = l{1} /\
+      DKCp.lsb{1} = Param.lsb{2} /\ 
+        Param.tbl{2} = map0 /\
+      (*(forall k, 0 <= k < i{1} => k = Param.l{2} => oget Param.kpub{2}.[(k,Param.lsb{2})] = (witness,witness)) /\
+      (forall k, 0 <= k < i{1} => k = DKCp.l{1} => oget DKCp.kpub{1}.[(k,DKCp.lsb{1})] = witness) /\*)
+      (forall k, 0 <= k < i{1} => k = Param.l{2} => oget DKCp.kpub{1}.[(k,DKCp.lsb{1})] = kw2w (fst (oget Param.kpub{2}.[(k,Param.lsb{2})])) Param.lsb{2}) /\
+      (forall k b, 0 <= k < i{1} => k <> Param.l{2} => oget DKCp.kpub{1}.[(k,b)] = kw2w (fst (oget Param.kpub{2}.[(k,b)])) b) /\
+      (*(forall k, 0 <= k < i{1} => k = Param.l{2} => snd (oget Param.kpub{2}.[(k,Param.lsb{2})]) = Param.lsb{2}) /\*)
+      (forall k b, 0 <= k < i{1} => snd (oget Param.kpub{2}.[(k,b)]) = b) /\
       (forall k, 0 <= k < i{1} => k = Param.l{2} => oget DKCp.kpub{1}.[(k,!Param.lsb{2})] = kw2w (fst (oget Param.kpub{2}.[(k,!Param.lsb{2})])) (!Param.lsb{2}))).
         
-        if; first by progress. print w2kw.
-        wp. rnd (fun w, fst (w2kw w)) (fun w, kw2w w (!Param.lsb{2})). wp. rnd{1}. rnd. skip; progress.
-        by rewrite Dword.dwordLsb_lossless.
-        simplify w2kw kw2w fst; smt tmo=15.
-        rewrite KW.Dword.mu_x_def Dword.dwordLsb_mu_x. cut ->: getlsb (kw2w kiR (!lsbL)) = !lsbL <=> true. simplify kw2w. rewrite get_setlsb. done. done.
+        if; first by progress. 
+        wp. rnd (fun w, fst (w2kw' w)) (fun w, kw2w' w (!Param.lsb{2})). wp. rnd. skip; progress.
+        (*by rewrite Dword.dwordLsb_lossless.*)
+        by rewrite w2kw'_kw2w'.  
+        rewrite KW.Dword.mu_x_def Dword.dwordLsb_mu_x. cut ->: getlsb (kw2w' kiR (!lsbL)) = !lsbL <=> true. simplify kw2w'. rewrite get_setlsb. done. done.
         by smt.
-        simplify w2kw kw2w fst; smt tmo=15. 
+        rewrite kw2w'_w2kw'. rewrite (Dword.lsb_dwordLsb (!lsbL) _). done. done. done. 
         idtac=>/#.
-        idtac=>/#. 
+        idtac=>/#.
         rewrite !getP => /#. 
+        rewrite !getP => /#.  
         rewrite !getP => /#. 
+        rewrite !getP ;smt.  
+
+    
+      auto; progress; first 2 by idtac=>/#. rewrite !getP => /#. 
+        rewrite !getP. case ((k, b1) = (i{2}, true)) => hc. rewrite !oget_some kw2w_w2kw. rewrite (Dword.lsb_dwordLsb (true) _). done. idtac=>/#. done. case ((k, b1) = (i{2}, false)) => hc'. rewrite !oget_some kw2w_w2kw. rewrite (Dword.lsb_dwordLsb (false) _). done. idtac=>/#. done. idtac=>/#.
+        rewrite !getP. case ((k, b1) = (i{2}, true)) => hc. rewrite oget_some. simplify w2kw snd. rewrite (Dword.lsb_dwordLsb (true) _). done. idtac=>/#. case ((k, b1) = (i{2}, false)) => hc'. rewrite oget_some. simplify w2kw snd. rewrite (Dword.lsb_dwordLsb (false) _). done. idtac=>/#. idtac=>/#. 
         rewrite !getP => /#. 
 
-      auto; progress; first 2 by idtac=>/#.
-        rewrite !getP. case ((k, true) = (i{2}, true)) => hc. simplify kw2w w2kw. rewrite oget_some. smt tmo=30. idtac=>/#. 
-        rewrite !getP. case ((k, false) = (i{2}, false)) => hc. simplify kw2w w2kw. rewrite oget_some. smt tmo=30. idtac=>/#. 
-        rewrite !getP => /#. 
-
-    wp; while (0 <= lp < boundl /\ b = true /\ ={i} /\ 0 <= i{1} <= bound /\ (b{1}, l{1}).`2 = lp /\ l{2} = lp /\
-      DKCp.used{1} = Param.used{2} /\ DKCp.used{1} = fset0 /\
-      DKCp.l{1} = Param.l{2} /\ DKCp.l{1} = lp /\ 
+    wp; while (={glob A} /\ 0 <= lp < bound /\ b{1} /\ ={i} /\ 0 <= i{1} <= bound /\ (b{1}, l{1}).`2 = lp /\ l{2} = lp /\
+      DKCp.used{1} = Param.used{2} /\ DKCp.used{1} = fset0 /\ DKCp.b{1} = b{1} /\ DKCp.b{1} /\
+      DKCp.l{1} = Param.l{2} /\ DKCp.l{1} = lp /\ Param.l{2} = l0{2} /\ DKCp.l{1} = l{1} /\
       DKCp.lsb{1} = Param.lsb{2} /\
-      Param.tbl{2} = map0 /\
+      Param.tbl{2} = map0 /\ 
       (forall k, 0 <= k < i{1} => oget DKCp.kpub{1}.[(k,false)] = W.zeros) /\
       (forall k, 0 <= k < i{1} => oget DKCp.kpub{1}.[(k,true)] = W.zeros) /\
       (forall k, 0 <= k < i{1} => oget Param.kpub{2}.[(k,false)] = (KW.zeros, false)) /\
       (forall k, 0 <= k < i{1} => oget Param.kpub{2}.[(k,true)] = (KW.zeros, true))).
       auto; progress; expect 6 by by rewrite ?getP => /#. 
 
-    auto; progress; last 8 by idtac=>/#.
-        by rewrite dK_ll. 
+    auto; progress; last 3 by idtac=>/#.
         by smt. 
         by rewrite map0P =>/#.
         by rewrite map0P =>/#.
         by rewrite map0P =>/#.
+        by rewrite map0P =>/#.
+        by smt.
+        by idtac=>/#.
+        by idtac=>/#.
+        by idtac=>/#.
+        by idtac=>/#. 
+        by rewrite w2kw'_kw2w'. 
+        rewrite KW.Dword.mu_x_def Dword.dwordLsb_mu_x. cut ->: getlsb (kw2w' kR (lsb_R)) = lsb_R <=> true. simplify kw2w'. rewrite get_setlsb. done. done. 
+        by smt.
+        rewrite kw2w'_w2kw'. by rewrite (Dword.lsb_dwordLsb (lsb_R) _). done.  
+        rewrite kw2w_w2kw'. by rewrite (Dword.lsb_dwordLsb (lsb_R) _). done.  
+        by rewrite (Dword.lsb_dwordLsb (lsb_R) _).  
+        rewrite H22 => /#. 
+        wp. 
 
-    wp. 
+    call (_: 
+  0 <= lp < bound /\
+  DKCp.used{1} = Param.used{2} /\
+  DKCp.b{1} /\
+  DKCp.l{1} = Param.l{2} /\
+  DKCp.l{1} = lp /\
+  DKCp.lsb{1} = Param.lsb{2} /\
+  DKCp.ksec{1} = kw2w PRFr_Wrapped.k{2} Param.lsb{2} /\
+  getlsb DKCp.ksec{1} = DKCp.lsb{1} /\
+  Param.tbl{2} = map0 /\
+  oget DKCp.kpub{1}.[(DKCp.l{1}, DKCp.lsb{1})] =
+        kw2w (fst (oget Param.kpub{2}.[(Param.l{2}, Param.lsb{2})])) Param.lsb{2} /\
+      (*snd (oget Param.kpub{2}.[(Param.l{2}, Param.lsb{2})]) = Param.lsb{2} /\*)
+  (forall (k : int) (b0 : bool),
+     0 <= k < bound =>
+     k <> Param.l{2} =>
+     oget DKCp.kpub{1}.[(k, b0)] =
+     kw2w (fst (oget Param.kpub{2}.[(k, b0)])) b0) /\
+  (forall (k : int) (b0 : bool),
+     0 <= k < bound =>
+     snd (oget Param.kpub{2}.[(k, b0)]) = b0) /\
+  (forall (k : int),
+    0 <= k < bound =>
+    k = Param.l{2} =>
+    oget DKCp.kpub{1}.[(k, !Param.lsb{2})] =
+    kw2w (fst (oget Param.kpub{2}.[(k, !Param.lsb{2})])) (!Param.lsb{2}))).
+
+    proc.
+    case (! mem DKCp.used{1} q{1}.`5 && 0 <= q{1}.`2.`1 /\       
+    q{1}.`2.`1 < q{1}.`3.`1 &&                 
+    q{1}.`3.`1 < q{1}.`4.`1 &&      q{1}.`4.`1 < bound /\             
+    q{1}.`4 <> (DKCp.l{1}, DKCp.lsb{1})); last first.
+
+      rcondf{1} 3; first by auto. 
+      rcondf{2} 3; first by auto. 
+      by auto.
+
+      rcondt{1} 3; first by auto. 
+      rcondt{2} 3; first by auto.
+ 
+      case (q{1}.`1).
+        rcondt{1} 8. auto => /#. 
+        rcondt{2} 8. auto. 
+
+    case (q{2}.`2 = (Param.l{2}, Param.lsb{2})).
+        rcondt{2} 9. progress. auto. 
+        inline PRFr_Wrapped.f. 
+        wp. rnd. wp. skip. progress. 
+        by rewrite H14 H3 => /#.   
+
+          cut ->: q{2}.`3 = (q{2}.`3.`1,q{2}.`3.`2) by idtac=>/#. rewrite H4 => /#.
+          simplify PrfDKC.E. simplify PRF.F. rewrite H14 /=. congr. congr. congr. rewrite w2kw_kw2w => /#. cut ->: q{2}.`3 = (q{2}.`3.`1,q{2}.`3.`2) by idtac=>/#. rewrite H4. idtac=>/#. idtac=>/#. rewrite w2kw_kw2w =>/#. 
+
+    case (q{2}.`3 = (Param.l{2}, Param.lsb{2})).
+        rcondf{2} 9. progress. auto. rcondt{2} 9. progress. auto. 
+        inline PRFr_Wrapped.f.
+        wp. rnd. wp. skip. progress.
+        cut ->: q{2}.`2 = (q{2}.`2.`1,q{2}.`2.`2) by idtac=>/#. rewrite H4 => /#.
+        by rewrite H15 H3 => /#. 
+        simplify PrfDKC.E. simplify PRF.F. cut ->: q{2}.`2 = (Param.l{2}, Param.lsb{2}) <=> false by idtac=>/#. rewrite H15 /=. congr. congr. congr. cut ->: q{2}.`2 = (q{2}.`2.`1,q{2}.`2.`2) by idtac=>/#. rewrite H4. idtac=>/#. idtac=>/#. rewrite w2kw_kw2w =>/#. rewrite w2kw_kw2w => /#. 
+
+    rcondf{2} 9. progress. auto. 
+    rcondf{2} 9. auto.
+    (*case (q{2}.`2.`1 = Param.l{2}).*)    
+
+    wp. rnd. wp. skip. progress.
+      by idtac=>/#.
+      by idtac=>/#.
+      cut ->: q{2}.`2 = (Param.l{2}, Param.lsb{2}) <=> false by idtac=>/#. cut ->: q{2}.`3 = (Param.l{2}, Param.lsb{2}) <=> false by idtac=>/#. simplify. simplify E. congr. congr. congr. cut ->: q{2}.`2 = (q{2}.`2.`1,q{2}.`2.`2) by idtac=>/#. by smt. by smt. 
 
 
+    (********************)
+    (* !rn *)
+    (********************)
+
+    rcondf{1} 8. progress. auto. progress. idtac=>/#.
+    rcondf{2} 8. progress. auto.
+
+    case (q{2}.`2 = (Param.l{2}, Param.lsb{2})).
+        rcondt{2} 8. progress. auto. 
+        inline PRFr_Wrapped.f. 
+        wp. skip. progress. 
+        by rewrite H14 H3 => /#.   
+
+          cut ->: q{2}.`3 = (q{2}.`3.`1,q{2}.`3.`2) by idtac=>/#. rewrite H4 => /#.
+          simplify PrfDKC.E. simplify PRF.F. rewrite H14 /=. congr. congr. congr. rewrite w2kw_kw2w => /#. cut ->: q{2}.`3 = (q{2}.`3.`1,q{2}.`3.`2) by idtac=>/#. rewrite H4. idtac=>/#. idtac=>/#. rewrite w2kw_kw2w =>/#. idtac=>/#.
+
+    case (q{2}.`3 = (Param.l{2}, Param.lsb{2})).
+        rcondf{2} 8. progress. auto. rcondt{2} 8. progress. auto. 
+        inline PRFr_Wrapped.f.
+        wp. skip. progress.
+        cut ->: q{2}.`2 = (q{2}.`2.`1,q{2}.`2.`2) by idtac=>/#. rewrite H4 => /#.
+        by rewrite H15 H3 => /#. 
+        simplify PrfDKC.E. simplify PRF.F. cut ->: q{2}.`2 = (Param.l{2}, Param.lsb{2}) <=> false by idtac=>/#. rewrite H15 /=. congr. congr. congr. cut ->: q{2}.`2 = (q{2}.`2.`1,q{2}.`2.`2) by idtac=>/#. rewrite H4. idtac=>/#. idtac=>/#. rewrite w2kw_kw2w =>/#. rewrite w2kw_kw2w => /#. idtac=>/#.
+
+    rcondf{2} 8. progress. auto. 
+    rcondf{2} 8. auto.
+    (*case (q{2}.`2.`1 = Param.l{2}).*)    
+
+    wp. skip. progress.
+      by idtac=>/#.
+      by idtac=>/#.
+      cut ->: q{2}.`2 = (Param.l{2}, Param.lsb{2}) <=> false by idtac=>/#. cut ->: q{2}.`3 = (Param.l{2}, Param.lsb{2}) <=> false by idtac=>/#. simplify. simplify E. congr. congr. congr. cut ->: q{2}.`2 = (q{2}.`2.`1,q{2}.`2.`2) by idtac=>/#. by smt. by smt. idtac=>/#.
+
+  skip. progress => /#.
+  qed.
+  
+equiv false_key lp (A <:  Adv_DKC_t{Param,DKCp,PRFr_Wrapped,RandomFunction}):
+    DKCSecurity.Game(DKC_O,A).game ~
+    IND(RandomFunction,D(A)).main : ={glob A} /\ 0 <= lp < bound /\ !b{1} /\ l{1} = lp /\ l{2} = lp
+                               ==> ={res}.
+
+    proof.
+      proc. 
+      inline PRFr_Wrapped.init RandomFunction.init D(A, RandomFunction).distinguish DKC_O.initialize. swap{1} 13 -1.
+      seq 12 3 : (={glob A} /\ 0 <= lp < bound /\ !b{1} /\ (b{1}, l{1}).`2 = lp /\ l{2} = lp /\
+      DKCp.used{1} = Param.used{2} /\ DKCp.used{1} = fset0 /\ DKCp.b{1} = b{1} /\ !DKCp.b{1} /\
+      DKCp.l{1} = Param.l{2} /\ DKCp.l{1} = lp /\ Param.l{2} = l0{2} /\ DKCp.l{1} = l{1} /\
+      DKCp.lsb{1} = Param.lsb{2} /\ lsb{1} = DKCp.lsb{1} /\ lsb{2} = Param.lsb{2} /\ (*getlsb DKCp.ksec{1} = DKCp.lsb{1} /\*)
+      Param.tbl{2} = map0 /\
+      RandomFunction.m{2} = map0 /\
+      (*oget Param.kpub{2}.[(Param.l{2},Param.lsb{2})] = (witness,witness) /\
+      oget DKCp.kpub{1}.[(DKCp.l{1},DKCp.lsb{1})] = witness /\*)
+      oget DKCp.kpub{1}.[(DKCp.l{1},DKCp.lsb{1})] = kw2w (fst (oget Param.kpub{2}.[(Param.l{2},Param.lsb{2})])) Param.lsb{2} /\
+      (*snd (oget Param.kpub{2}.[(Param.l{2},Param.lsb{2})]) = Param.lsb{2} /\*)
+      (forall k b, 0 <= k < bound => k <> Param.l{2} => oget DKCp.kpub{1}.[(k,b)] = kw2w (fst (oget Param.kpub{2}.[(k,b)])) b) /\
+      (forall k b, 0 <= k < bound => snd (oget Param.kpub{2}.[(k,b)]) = b) /\
+      (forall k, 0 <= k < bound => k = Param.l{2} => oget DKCp.kpub{1}.[(k,!Param.lsb{2})] = kw2w (fst (oget Param.kpub{2}.[(k,!Param.lsb{2})])) (!Param.lsb{2}))
+
+
+
+    );   
+      inline DKC_O.initialize D(A, RandomFunction).initialize.
+        
+    
+        (*swap{2} 1 11.
+        wp. rnd (fun w, fst (w2kw' w)) (fun w, kw2w' w (Param.lsb{2})).*)
+    
+        wp; while (={glob A} /\ 0 <= lp < bound /\ !b{1} /\ ={i} /\ 0 <= i{1} <= bound /\ (b{1}, l{1}).`2 = lp /\ l{2} = lp /\
+      DKCp.used{1} = Param.used{2} /\ DKCp.used{1} = fset0 /\ DKCp.b{1} = b{1} /\ !DKCp.b{1} /\
+      DKCp.l{1} = Param.l{2} /\ DKCp.l{1} = lp /\ Param.l{2} = l0{2} /\ DKCp.l{1} = l{1} /\
+      DKCp.lsb{1} = Param.lsb{2} /\ 
+        Param.tbl{2} = map0 /\ 
+      (*(forall k, 0 <= k < i{1} => k = Param.l{2} => oget Param.kpub{2}.[(k,Param.lsb{2})] = (witness,witness)) /\
+      (forall k, 0 <= k < i{1} => k = DKCp.l{1} => oget DKCp.kpub{1}.[(k,DKCp.lsb{1})] = witness) /\*)
+      (forall k, 0 <= k < i{1} => k = Param.l{2} => oget DKCp.kpub{1}.[(k,DKCp.lsb{1})] = kw2w (fst (oget Param.kpub{2}.[(k,Param.lsb{2})])) Param.lsb{2}) /\
+      (forall k b, 0 <= k < i{1} => k <> Param.l{2} => oget DKCp.kpub{1}.[(k,b)] = kw2w (fst (oget Param.kpub{2}.[(k,b)])) b) /\
+      (*(forall k, 0 <= k < i{1} => k = Param.l{2} => snd (oget Param.kpub{2}.[(k,Param.lsb{2})]) = Param.lsb{2}) /\*)
+      (forall k b, 0 <= k < i{1} => snd (oget Param.kpub{2}.[(k,b)]) = b) /\
+      (forall k, 0 <= k < i{1} => k = Param.l{2} => oget DKCp.kpub{1}.[(k,!Param.lsb{2})] = kw2w (fst (oget Param.kpub{2}.[(k,!Param.lsb{2})])) (!Param.lsb{2}))).
+        
+        if; first by progress. 
+        wp. rnd (fun w, fst (w2kw' w)) (fun w, kw2w' w (!Param.lsb{2})). wp. rnd. skip; progress.
+        (*by rewrite Dword.dwordLsb_lossless.*)
+        by rewrite w2kw'_kw2w'.  
+        rewrite KW.Dword.mu_x_def Dword.dwordLsb_mu_x. cut ->: getlsb (kw2w' kiR (!lsbL)) = !lsbL <=> true. simplify kw2w'. rewrite get_setlsb. done. done.
+        by smt.
+        rewrite kw2w'_w2kw'. rewrite (Dword.lsb_dwordLsb (!lsbL) _). done. done. done. 
+        idtac=>/#.
+        idtac=>/#.
+        rewrite !getP => /#. 
+        rewrite !getP => /#.  
+        rewrite !getP => /#. 
+        rewrite !getP ;smt.  
 
     
-  qed.
+      auto; progress; first 2 by idtac=>/#. rewrite !getP => /#. 
+        rewrite !getP. case ((k, b1) = (i{2}, true)) => hc. rewrite !oget_some kw2w_w2kw. rewrite (Dword.lsb_dwordLsb (true) _). done. idtac=>/#. done. case ((k, b1) = (i{2}, false)) => hc'. rewrite !oget_some kw2w_w2kw. rewrite (Dword.lsb_dwordLsb (false) _). done. idtac=>/#. done. idtac=>/#.
+        rewrite !getP. case ((k, b1) = (i{2}, true)) => hc. rewrite oget_some. simplify w2kw snd. rewrite (Dword.lsb_dwordLsb (true) _). done. idtac=>/#. case ((k, b1) = (i{2}, false)) => hc'. rewrite oget_some. simplify w2kw snd. rewrite (Dword.lsb_dwordLsb (false) _). done. idtac=>/#. idtac=>/#. 
+        rewrite !getP => /#. 
 
-equiv false_key l b (A <:  Adv_DKC_t):
-    DKCSecurity.Game(DKC,A).game ~
-    IND(RandomFunction,D(A)).main : 0 <= l{1} < bound && b{1} = false
-                               ==> ={res}.
-    proof.
-      proc. inline DKC.initialize PRFr_Wrapped.init D(A,PRFr_Wrapped).distinguish.
-      admit.
-    qed.
+    wp; while (={glob A} /\ 0 <= lp < bound /\ !b{1} /\ ={i} /\ 0 <= i{1} <= bound /\ (b{1}, l{1}).`2 = lp /\ l{2} = lp /\
+      DKCp.used{1} = Param.used{2} /\ DKCp.used{1} = fset0 /\ DKCp.b{1} = b{1} /\ !DKCp.b{1} /\
+      DKCp.l{1} = Param.l{2} /\ DKCp.l{1} = lp /\ Param.l{2} = l0{2} /\ DKCp.l{1} = l{1} /\
+      DKCp.lsb{1} = Param.lsb{2} /\
+      Param.tbl{2} = map0 /\ 
+      (forall k, 0 <= k < i{1} => oget DKCp.kpub{1}.[(k,false)] = W.zeros) /\
+      (forall k, 0 <= k < i{1} => oget DKCp.kpub{1}.[(k,true)] = W.zeros) /\
+      (forall k, 0 <= k < i{1} => oget Param.kpub{2}.[(k,false)] = (KW.zeros, false)) /\
+      (forall k, 0 <= k < i{1} => oget Param.kpub{2}.[(k,true)] = (KW.zeros, true))).
+      auto; progress; expect 6 by by rewrite ?getP => /#. 
+
+    auto; progress; last 3 by idtac=>/#.
+        by smt. 
+        by rewrite map0P =>/#.
+        by rewrite map0P =>/#.
+        by rewrite map0P =>/#.
+        by rewrite map0P =>/#.
+        by smt.
+        by idtac=>/#.
+        by idtac=>/#.
+        by idtac=>/#.
+        by idtac=>/#. 
+        rewrite H22 => /#. 
+        wp. 
+
+    call (_ : 
+  0 <= lp < bound /\
+  DKCp.used{1} = Param.used{2} /\
+  !DKCp.b{1} /\
+  DKCp.l{1} = Param.l{2} /\
+  DKCp.l{1} = lp /\
+  DKCp.lsb{1} = Param.lsb{2} /\
+  getlsb DKCp.ksec{1} = DKCp.lsb{1} /\
+  getlsb DKCp.ksec{1} = DKCp.lsb{1} /\
+  oget DKCp.kpub{1}.[(DKCp.l{1}, DKCp.lsb{1})] =
+  kw2w (fst (oget Param.kpub{2}.[(Param.l{2}, Param.lsb{2})])) Param.lsb{2} /\
+  (forall (k : int) (b0 : bool),
+     0 <= k < bound =>
+     k <> Param.l{2} =>
+     oget DKCp.kpub{1}.[(k, b0)] =
+     kw2w (fst (oget Param.kpub{2}.[(k, b0)])) b0) /\
+  (forall (k : int) (b0 : bool),
+     0 <= k < bound => snd (oget Param.kpub{2}.[(k, b0)]) = b0) /\
+  (forall (k : int),
+    0 <= k < bound =>
+    k = Param.l{2} =>
+    oget DKCp.kpub{1}.[(k, !Param.lsb{2})] =
+    kw2w (fst (oget Param.kpub{2}.[(k, !Param.lsb{2})])) (!Param.lsb{2}))).
+
+    proc.
+    
+    case (! mem DKCp.used{1} q{1}.`5 && 0 <= q{1}.`2.`1 /\       
+    q{1}.`2.`1 < q{1}.`3.`1 &&                 
+    q{1}.`3.`1 < q{1}.`4.`1 &&      q{1}.`4.`1 < bound /\             
+    q{1}.`4 <> (DKCp.l{1}, DKCp.lsb{1})); last first.
+
+      rcondf{1} 3; first by auto. 
+      rcondf{2} 3; first by auto. 
+      by auto.
+
+      rcondt{1} 3; first by auto. 
+      rcondt{2} 3; first by auto.
+ 
+      case (q{1}.`1).
+        rcondt{1} 8. auto => /#. 
+        rcondt{2} 8. auto. 
+
+    case (q{2}.`2 = (Param.l{2}, Param.lsb{2})).
+        rcondt{2} 9. progress. auto. 
+        inline RandomFunction.f.
+        rcondt{2} 10. auto.  progress. admit. 
+        wp. rnd{2} (fun w, fst (w2kw' w)) (fun w, kw2w' w (!Param.lsb{2})). wp. rnd. wp. skip. progress. 
+          by smt.
+          by rewrite H13 H2 => /#.   
+
+          cut ->: q{2}.`3 = (q{2}.`3.`1,q{2}.`3.`2) by idtac=>/#. rewrite H3 => /#.
+          simplify PrfDKC.E. simplify PRF.F. rewrite H13 /=. rewrite getP. simplify. rewrite oget_some. admit. cut ->: q{2}.`3 = (q{2}.`3.`1,q{2}.`3.`2) by idtac=>/#. rewrite H3. idtac=>/#. idtac=>/#. rewrite w2kw_kw2w =>/#. 
+
+    case (q{2}.`3 = (Param.l{2}, Param.lsb{2})).
+        rcondf{2} 9. progress. auto. rcondt{2} 9. progress. auto. 
+        inline RandomFunction.f.
+        rcondt{2} 10. auto.  progress. admit.
+        wp. rnd{2}. wp. rnd. wp. skip. progress.
+        by smt.
+        cut ->: q{2}.`2 = (q{2}.`2.`1,q{2}.`2.`2) by idtac=>/#. rewrite H3 => /#.
+        by rewrite H14 H2 => /#. 
+        simplify PrfDKC.E. simplify PRF.F. cut ->: q{2}.`2 = (Param.l{2}, getlsb DKCp.ksec{1}) <=> false by idtac=>/#. rewrite H14 /=. congr. congr. congr. cut ->: q{2}.`2 = (q{2}.`2.`1,q{2}.`2.`2) by idtac=>/#. rewrite H3. idtac=>/#. idtac=>/#. rewrite w2kw_kw2w =>/#. admit. 
+
+    rcondf{2} 9. progress. auto. 
+    rcondf{2} 9. auto.
+
+    wp. rnd. wp. skip. progress.
+      by idtac=>/#.
+      by idtac=>/#.
+      cut ->: q{2}.`2 = (Param.l{2}, getlsb DKCp.ksec{1}) <=> false by idtac=>/#. cut ->: q{2}.`3 = (Param.l{2}, getlsb DKCp.ksec{1}) <=> false by idtac=>/#. simplify. simplify E. congr. congr. congr. cut ->: q{2}.`2 = (q{2}.`2.`1,q{2}.`2.`2) by idtac=>/#. by smt. by smt. 
+
+
+    (********************)
+    (* !rn *)
+    (********************)
+
+    case (q{2}.`2 = (Param.l{2}, Param.lsb{2})).
+
+    rcondt{1} 8. progress. auto. progress. idtac=>/#. 
+    rcondf{2} 8. progress. auto.
+
+    
+        rcondt{2} 8. progress. auto. 
+        inline RandomFunction.f.
+        rcondt{2} 9. auto.  progress. admit.
+        wp. rnd{1}. rnd{2}. wp. skip. progress. 
+        by smt. by smt. by rewrite H13 H2 => /#.   
+
+          cut ->: q{2}.`3 = (q{2}.`3.`1,q{2}.`3.`2) by idtac=>/#. rewrite H3 => /#.
+          simplify PrfDKC.E. simplify PRF.F. rewrite H13 /=. congr. congr. admit. congr. cut ->: q{2}.`3 = (q{2}.`3.`1,q{2}.`3.`2) by idtac=>/#. rewrite H3. idtac=>/#. idtac=>/#. rewrite w2kw_kw2w =>/#. admit. 
+
+    case (q{2}.`3 = (Param.l{2}, Param.lsb{2})).
+        rcondt{1} 8. progress. auto. progress. idtac=>/#. 
+    rcondf{2} 8. progress. auto.
+        rcondf{2} 8. progress. auto. rcondt{2} 8. progress. auto. 
+        inline RandomFunction.f. rcondt{2} 9. auto.  progress. admit.
+        wp. rnd{1}skip. progress.
+        cut ->: q{2}.`2 = (q{2}.`2.`1,q{2}.`2.`2) by idtac=>/#. rewrite H4 => /#.
+        by rewrite H15 H3 => /#. 
+        simplify PrfDKC.E. simplify PRF.F. cut ->: q{2}.`2 = (Param.l{2}, Param.lsb{2}) <=> false by idtac=>/#. rewrite H15 /=. congr. congr. congr. cut ->: q{2}.`2 = (q{2}.`2.`1,q{2}.`2.`2) by idtac=>/#. rewrite H4. idtac=>/#. idtac=>/#. rewrite w2kw_kw2w =>/#. rewrite w2kw_kw2w => /#. idtac=>/#.
+
+    rcondf{2} 8. progress. auto. 
+    rcondf{2} 8. auto.
+    (*case (q{2}.`2.`1 = Param.l{2}).*)    
+
+    wp. skip. progress.
+      by idtac=>/#.
+      by idtac=>/#.
+      cut ->: q{2}.`2 = (Param.l{2}, Param.lsb{2}) <=> false by idtac=>/#. cut ->: q{2}.`3 = (Param.l{2}, Param.lsb{2}) <=> false by idtac=>/#. simplify. simplify E. congr. congr. congr. cut ->: q{2}.`2 = (q{2}.`2.`1,q{2}.`2.`2) by idtac=>/#. by smt. by smt. idtac=>/#.
+
+
+
+
+  qed.
 
     
 lemma PrfDKC_secure : forall (A <: Adv_DKC_t) &m i, 0 <= i < bound =>
